HelloTypeSystem/Meta.lean
@@ -9,3 +9,5 @@ import «HelloTypeSystem».Meta.TypingML1
 
 import «HelloTypeSystem».Meta.EvalML2
 import «HelloTypeSystem».Meta.TypingML2
+
+import «HelloTypeSystem».Meta.ML3
