HelloTypeSystem/Meta/ML3/Eval.lean
@@ -1,0 +1,181 @@
+import HelloTypeSystem.ML3
+
+namespace HelloTypeSystem.ML3
+
+/-!
+# EvalML3のメタ定理
+-/
+
+/-
+## EvalML3における判断の導出例
+
+### 練習問題5.1
+-/
+
+example : Evaluation Env.nil (.Let "sq" (.Fn "x" ("x" * "x")) ((.App "sq" 3) + (.App "sq" 4))) 25 :=
+  (.Let .Fn
+    (.Add
+      (.App .Var .Int
+        (.Mul (.Var) (.Var))
+      )
+      (.App .Var .Int
+        (.Mul (.Var) (.Var))
+      )
+    )
+  )
+
+example : Evaluation Env.nil (.Let "sm" (.Fn "f" ((.App "f" 3) + (.App "f" 4))) (.App "sm" (.Fn "x" ("x" * "x")))) 25 :=
+  (.Let .Fn
+    (.App .Var .Fn
+      (.Add
+        (.App .Var .Int
+          (.Mul (.Var) (.Var))
+        )
+        (.App .Var .Int
+          (.Mul (.Var) (.Var))
+        )
+      )
+    )
+  )
+
+example : Evaluation Env.nil
+  (
+    (.Let "twice" (.Fn "f" (.Fn "x" (.App "f" (.App "f" "x"))))
+      /- in -/
+      (.App (.App "twice" (.Fn "x" ("x" * "x"))) 2)
+    )
+  )
+  16
+:=
+  (.Let .Fn
+    (.App
+      (.App .Var .Fn .Fn)
+      (.Int)
+      (.App
+        (.VarIr .Var)
+        (.App
+          (.VarIr .Var)
+          (.Var)
+          (.Mul .Var .Var)
+        )
+        (.Mul .Var .Var)
+      )
+    )
+  )
+
+example : Evaluation Env.nil
+  (
+    (.Let "compose"
+      /- := -/
+      (.Fn "f"
+        (.Fn "g"
+          (.Fn "x"
+            (.App "f" (.App "g" "x"))
+          )
+        )
+      )
+      /- in -/
+      (.Let "p" (.Fn "x" ("x" * "x"))
+        /- in -/
+        (.Let "q" (.Fn "x" ("x" + 4))
+          /- in -/
+          (.App (.App (.App "compose" "p") "q") 4) -- compose p q 4
+        )
+      )
+    )
+  )
+  64
+:=
+  -- let compose = fun ... in
+  (.Let .Fn
+    -- let p = fun ... in
+    (.Let .Fn
+      -- let q = fun ... in
+      (.Let .Fn
+        -- compose p q 4
+        (.App
+          -- compose p q
+          (.App
+            -- compose p
+            (.App
+              (.VarIr (.VarIr .Var)) -- compose
+              (.VarIr .Var)          -- p
+              (.Fn) -- compose p
+            )
+            (.Var) -- q
+            (.Fn) -- (compose p) q
+          )
+          (.Int) -- 4
+          -- f (g x)
+          (.App
+            (.VarIr (.VarIr .Var))
+            -- g x = q x = x + 4
+            (.App (.VarIr .Var) (.Var) (.Add .Var .Int))
+            (.Mul .Var .Var) -- x * x = p x = f x
+          )
+        )
+      )
+    )
+  )
+
+/-!
+## EvalML3の評価の一意性
+-/
+
+/--
+EvalML3の評価の一意性（\[基礎概念,§5.7] 定理5.2）
+-/
+theorem eval_value_uniq {e : Expr} {E : Env} {v : Value} (d : Evaluation E e v) : {v' : Value} → Evaluation E e v' → v = v' :=
+  d.induction
+    (motive := fun E e v => ∀ {v' : Value}, Evaluation E e v' → v = v')
+    (fun .Int  => rfl)
+    (fun .Bool => rfl)
+    (fun .Var  => rfl)
+    (fun _ d _ (.VarIr d') => d d')
+    (fun d₁ d₂ h _ (.Add d₁' d₂' h') =>
+      have h₁ := d₁ d₁' |> Value.Z.inj
+      have h₂ := d₂ d₂' |> Value.Z.inj
+      congrArg Value.Z (h ▸ h₂ ▸ h₁ ▸ h')
+    )
+    (fun d₁ d₂ h _ (.Sub d₁' d₂' h') =>
+      have h₁ := d₁ d₁' |> Value.Z.inj
+      have h₂ := d₂ d₂' |> Value.Z.inj
+      congrArg Value.Z (h ▸ h₂ ▸ h₁ ▸ h')
+    )
+    (fun d₁ d₂ h _ (.Mul d₁' d₂' h') =>
+      have h₁ := d₁ d₁' |> Value.Z.inj
+      have h₂ := d₂ d₂' |> Value.Z.inj
+      congrArg Value.Z (h ▸ h₂ ▸ h₁ ▸ h')
+    )
+    (fun d₁ d₂ h _ d' =>
+      match d' with
+      | .LTT _ _ _      => rfl
+      | .LTF d₁' d₂' h' =>
+          have h₁ := d₁ d₁' |> Value.Z.inj
+          have h₂ := d₂ d₂' |> Value.Z.inj
+          absurd h (h₂ ▸ h₁ ▸ h')
+    )
+    (fun d₁ d₂ h _ d' =>
+      match d' with
+      | .LTF _ _ _      => rfl
+      | .LTT d₁' d₂' h' =>
+          have h₁ := d₁ d₁' |> Value.Z.inj
+          have h₂ := d₂ d₂' |> Value.Z.inj
+          absurd (h₂ ▸ h₁ ▸ h') h
+    )
+    (fun d₁ d₂ _ d' =>
+      match d' with
+      | .IfT _   d₂' => d₂ d₂'
+      | .IfF d₁' _   => d₁ d₁' |> Value.B.inj |> Bool.noConfusion
+    )
+    (fun d₁ d₂ _ d' =>
+      match d' with
+      | .IfF _   d₂' => d₂ d₂'
+      | .IfT d₁' _   => d₁ d₁' |> Value.B.inj |> Bool.noConfusion
+    )
+    (fun d₁ d₂ _ (.Let d₁' d₂') => d₂ (d₁ d₁' ▸ d₂'))
+    (fun .Fn => rfl)
+    (fun d₁ d₂ d₀ _ (.App d₁' d₂' d₀') =>
+      have ⟨h₁, h₂, h₃⟩ := d₁ d₁' |> Value.Cls.inj
+      d₀ <| h₃ ▸ h₂ ▸ h₁ ▸ d₂ d₂' ▸ d₀'
+    )
